src/algebraic/AG_to_RG.v
@@ -61,4 +61,4 @@ Coercion AG_to_RG : AG >-> RG_unlE.
 Definition AG_equiv {A : Type} (ag1 ag2 : AG A) : Prop :=
     RG_equiv (AG_to_RG ag1) (AG_to_RG ag2).
 
-Notation "g1 A== g2" := (AG_equiv g1 g2) (at level 80).
+Notation "g1 ==A g2" := (AG_equiv g1 g2) (at level 80).
